Rego.Interpreter.fst
@@ -10,16 +10,22 @@ type intr=interpreter
 
 let make_new () = {
    rules = [];
-   scopes = []
+   scopes = [];
+   loop_exprs = [];
 }
 
-let rec eval_expr (e:expr) (i:intr)  : Tot (value*intr) =
+let rec eval_expr (e:expr) (i:intr)  : Tot (value*intr) 
+//(decreases expr)
+=
   match e with
   | Var v -> lookup_var v i
   | Value v -> (v, i)
   | Ast.Array elems -> eval_array_elems elems [] i
   | Ast.Set elems -> eval_set_elems elems [] i
   | Ast.Object fields -> eval_fields fields (Object []) i
+  | Ast.ArrayCompr query -> eval_query_stmts query.stmts (Value.Array []) i
+  | Ast.SetCompr query -> eval_query_stmts query.stmts (Value.Set []) i
+  | Ast.ObjectCompr query -> eval_query_stmts query.stmts (Value.Object []) i
   | _ -> (Undefined, i)
 
 and eval_array_elems (elems:list expr) (values:list value) (i:intr)  : Tot (value*intr)
@@ -54,9 +60,36 @@ and eval_fields (fields:list (expr*expr)) (obj:value) (i:intr)  : Tot (value*int
       match eval_expr value_expr i' with
       | (Undefined, i'') -> (Undefined, i'')
       | (vv, i'') -> eval_fields tl (insert_into_object obj kv vv) i''
-
-and lookup_var (ident:string) (i:intr)  : Tot (value*intr) (decreases ident) =
+  
+and lookup_var (ident:string) (i:intr)  : Tot (value*intr) 
+(decreases ident) 
+=
   (Undefined, i)
 
+and eval_query_stmts (stmts:list literalStmt) (out:value) (i:intr) : Tot (value*intr) 
+(decreases stmts)
+=
+  match stmts with
+  | hd::[] ->
+    (match hd.literal with
+    | ArrayComprOutput e -> 
+      let (v, i') = eval_expr e i in
+      (insert_into_array out v, i')
+    | SetComprOutput e -> 
+      let (v, i') = eval_expr e i in
+      (insert_into_set out v, i')
+    | ObjectComprOutput (ke, ve) -> 
+      let (kv, i') = eval_expr ke i in
+      let (vv, i'') = eval_expr ve i' in
+      (insert_into_object out kv vv, i')
+    | _ -> (Undefined, i))
+  | hd::tl ->
+    let (v, i') = match hd.literal with
+    | Expr e -> eval_expr e i
+    | _ -> (Undefined, i)
+    in eval_query_stmts tl out i' 
+  | [] -> (Undefined, i)
+ 
 let eval (i:intr) (e:Ast.expr) : (value*intr) =
   eval_expr e i
+
